Add Uint64 helpers

src/StandardLibrary/UInt.dfy
@@ -14,6 +14,7 @@ module StandardLibrary.UInt {
 
   const UINT16_LIMIT := 0x1_0000
   const UINT32_LIMIT := 0x1_0000_0000
+  const UINT64_LIMIT := 0x1_0000_0000_0000_0000
   const INT32_MAX_LIMIT := 0x8000_0000
   const INT64_MAX_LIMIT := 0x8000_0000_0000_0000
 
@@ -32,6 +33,13 @@ module StandardLibrary.UInt {
 
   type seq32<T> = s: seq<T> | HasUint32Len(s)
   type Uint8Seq32 = seq32<uint8>
+
+  predicate method HasUint64Len<T>(s: seq<T>) {
+    |s| < UINT64_LIMIT
+  }
+
+  type seq64<T> = s: seq<T> | HasUint64Len(s)
+  type Uint8Seq64 = seq64<uint8>
 
   function method UInt16ToSeq(x: uint16): (ret: seq<uint8>)
     ensures |ret| == 2
